added event times queue

snglswch/lucid_base.dfy
@@ -39,9 +39,10 @@ TODO:
 abstract module LucidBase {
    type bits = x : int | 0 <= x < 256                 // number must match
                                                       // the parameter T
+   const T : nat := 256
 
     type Event(==)
-
+    datatype EventTime = EventTime(time : bits, ghost natTime : nat)
     class State {
         constructor () 
             ensures fresh(this)
@@ -70,17 +71,65 @@ abstract module LucidBase {
     class Handlers {
         var state : State
         var event_queue : seq<Event>
+        var event_times : seq<EventTime>
+        var last_event_nattime : nat // the arrival time of the last event queued thus far
         var out_queue : seq<Event>
         
         // time-related state
         var time : bits
         ghost var natTime : nat
         ghost var lastNatTime : nat
-        
+
+        /******* event time predicates  *******/
+
+        ghost predicate TimeIsNonDecreasing(eventTimes: seq<EventTime>)
+        // natural event times are non decreasing
+        {
+            forall i :: 1 <= i < |eventTimes| ==> eventTimes[i].natTime >= eventTimes[i - 1].natTime
+        }    
+        ghost predicate TimestampIsCorrect(eventTimes: seq<EventTime>)
+        // bit event time equals natural event time mod T
+        {
+            forall i :: 0 <= i < |eventTimes| ==> eventTimes[i].time == eventTimes[i].natTime % T   
+        }
+        ghost predicate EventTimesBase(eventTimes: seq<EventTime>)
+        {
+            TimeIsNonDecreasing(eventTimes) && TimestampIsCorrect(eventTimes)
+        }
+        ghost predicate EventTimesInvariant(eventTimes: seq<EventTime>)
+        requires EventTimesBase(eventTimes)
+        ensures  EventTimesBase(eventTimes)
+
+
+        // predicate base_event_times()
+        //     reads this`event_times
+        //     {
+                
+        //     }
+
+
+        // this should: 
+        // always hold on q.pre_handler_contents
+        // hold on q.contents before and after handler execution
+        ghost predicate inter_event_invariant(s : State, es : seq<Event>, time : bits, natTime : nat, lastNatTime : nat)
+            reads s
+
+        // ghost predicate time_invariant()
+        //     reads this`time, this`natTime, this`lastNatTime
+
+        ghost predicate queue_invariant(s : State, es : seq<Event>, time : bits, natTime : nat, lastNatTime : nat)
+            reads this`event_queue
+            ensures inter_event_invariant(s, es, time, natTime, lastNatTime)
+
+
         constructor()
             ensures (fresh(state))
             ensures (this.event_queue == [])
-            ensures time_invariant()
+            ensures time == natTime % T
+            ensures natTime >= lastNatTime
+            ensures (|this.event_times| == |this.event_queue|)
+
+            // ensures time_invariant()
         //     // ensures (inter_event_invariant(state, event_queue))
         //     // ensures (empty_implies_inter(state, event_queue))
         //     {
@@ -90,82 +139,92 @@ abstract module LucidBase {
         //      time := 1;
         //     }
             
-        // this should: 
-        // always hold on q.pre_handler_contents
-        // hold on q.contents before and after handler execution
-        ghost predicate inter_event_invariant(s : State, es : seq<Event>)
-            reads s
-            reads this`time, this`natTime, this`lastNatTime
+        // run the program on event e and up to "r" recirculated events
+        method Run(e : Event, r : int)
+            modifies this.state, this`event_queue, this`out_queue, this`event_times,
+            this`natTime, this`time, this`lastNatTime
+            requires |event_queue| == |event_times|
+            requires time == natTime % T
+            requires natTime >= lastNatTime
+            requires inter_event_invariant(state, event_queue, this.time, this.natTime, this.lastNatTime)
+            // requires time_invariant()
+        {
+            var i := 0;
+            assert(inter_event_invariant(state, event_queue, this.time, this.natTime, this.lastNatTime));
+            // assert time_invariant();
+            while(i < r)
+            invariant inter_event_invariant(state, event_queue, this.time, this.natTime, this.lastNatTime)
+            invariant time == natTime % T
+            invariant natTime >= lastNatTime
+            invariant |event_queue| == |event_times|
+            // invariant time_invariant()
+            {
+                // call the user-defined "Dispatch" function to handle the event. 
+                // the effects of dispatch are to: 
+                // 1. change state values; 2. change queue contents (current event gets dequeued automatically, more may be added by generate).
+                if (event_queue != []){
+                    var e, new_event_queue := dequeue(event_queue);     
+                    var et, new_event_times := dequeue(event_times);   
+                    event_queue := new_event_queue;
+                    event_times := new_event_times;
+                    Dispatch(e, et);
+                }
+                i := i + 1;
+            }
+        }
 
-        ghost predicate time_invariant()
-            reads this`time, this`natTime, this`lastNatTime
 
 
         // A program must extend this function to handle events in a way that is 
         // consistent with the inter event invariant. 
         // Note that this function is not allowed to modify time variables.
-        method Dispatch(e : Event)
-            modifies this.state, this`event_queue, this`out_queue
-            requires time_invariant()
-            requires (inter_event_invariant(state, [e]+event_queue))
-            ensures time_invariant()
-            ensures inter_event_invariant(state, event_queue)
+        method Dispatch(e : Event, t : EventTime)
+            modifies this.state, this`event_queue, this`out_queue, this`event_times
+            // requires time_invariant()
+            requires time == natTime % T
+            requires natTime >= lastNatTime
+            requires |event_queue| == |event_times|
+
+            requires (inter_event_invariant(state, [e]+event_queue, this.time, this.natTime, this.lastNatTime))
+            // ensures time_invariant()
+            ensures time == natTime % T
+            ensures natTime >= lastNatTime
+            ensures |event_queue| == |event_times|
+            ensures inter_event_invariant(state, event_queue, this.time, this.natTime, this.lastNatTime)
             // ensures valid_generate(old(event_queue), event_queue)
 
         // The program has to exend this function to update the clock in a way that 
         // is consistent with its invariant.
-        method ClockTick()
-            modifies this`time, this`natTime, this`lastNatTime
-            requires time_invariant()
-            requires inter_event_invariant(state, event_queue)
-            ensures time_invariant()
-            ensures  inter_event_invariant(state, event_queue)
+        // method ClockTick()
+        //     modifies this`time, this`natTime, this`lastNatTime
+        //     requires time_invariant()
+        //     requires inter_event_invariant(state, event_queue, this.time, this.natTime, this.lastNatTime)
+        //     ensures time_invariant()
+        //     ensures  inter_event_invariant(state, event_queue, this.time, this.natTime, this.lastNatTime)
 
 
-        // Queue an event to be processed in the future. 
+        // Queue an event to be processed 1 time-unit after the last event in the queue. 
         method Generate(e : Event)
             modifies this`event_queue
+            modifies this`event_times
+            requires |event_queue| == |event_times|
+            ensures |event_queue| == |event_times|
             ensures (this.event_queue == old(this.event_queue) + [e])
             {
                 this.event_queue := this.event_queue + [e];
+                var nat_time := if (|event_times| == 0) then 1 else (event_times[|event_times| -1].natTime + 1);
+                var time  := if (|event_times| == 0) then 1 else ((event_times[|event_times| -1].time + 1) % T);
+                var event_time := EventTime(time, nat_time);
+                this.event_times := this.event_times + [event_time];
             }
         // Queue an event to send out into the network.
-        // I think this might be a noop.
+        // this might be a noop?
         method Send(e : Event) 
             modifies this`out_queue
             ensures out_queue == old(out_queue) + [e]
             {
                 out_queue := out_queue + [e];
             }
-
-        // run the program on event e and up to "r" recirculated events
-        method Run(e : Event, r : int)
-            modifies this.state, this`event_queue, this`out_queue, 
-            this`natTime, this`time, this`lastNatTime
-            requires inter_event_invariant(state, event_queue)
-            requires time_invariant()
-        {
-            var i := 0;
-            assert(inter_event_invariant(state, event_queue));
-            assert time_invariant();
-            while(i < r)
-            invariant inter_event_invariant(state, event_queue)
-            invariant time_invariant()
-            {
-                // first, call the user-defined "Dispatch" function to handle the event. 
-                // the effects of dispatch are to: 
-                // 1. change state values; 2. change queue contents (current event gets dequeued automatically, more may be added by generate).
-                if (event_queue != []){
-                    var e, new_event_queue := dequeue(event_queue);        
-                    event_queue := new_event_queue;
-                    Dispatch(e);
-                }
-                // now, call the user function to update time in a
-                // way that is consistent with the program's assumptions
-                ClockTick();
-                i := i + 1;
-            }
-        }
 
 
         // function seq_contains(es : seq<Event>, f : Event -> bool) : bool
@@ -185,7 +244,7 @@ abstract module LucidBase {
         }
 
         // private helpers
-        method dequeue(es : seq<Event>) returns (e : Event, es2 : seq<Event>)
+        method dequeue<T>(es : seq<T>) returns (e : T, es2 : seq<T>)
             requires (|es| > 0)
             ensures (es == [e] + es2)
             {e := es[0]; es2 := es[1..];}
